<?xml version="1.0"?>
<rdf:RDF xmlns="http://www.semanticweb.org/gianpietro/ontologies/2022/6/untitled-ontology-39#"
     xml:base="http://www.semanticweb.org/gianpietro/ontologies/2022/6/untitled-ontology-39"
     xmlns:owl="http://www.w3.org/2002/07/owl#"
     xmlns:rdf="http://www.w3.org/1999/02/22-rdf-syntax-ns#"
     xmlns:xml="http://www.w3.org/XML/1998/namespace"
     xmlns:xsd="http://www.w3.org/2001/XMLSchema#"
     xmlns:rdfs="http://www.w3.org/2000/01/rdf-schema#"
     xmlns:oasis="http://www.dmi.unict.it/oasis.owl#"
     xmlns:terms="http://purl.org/dc/terms/"
     xmlns:untitled-ontology-39="http://www.semanticweb.org/gianpietro/ontologies/2022/6/untitled-ontology-39#">
    <owl:Ontology rdf:about="http://www.semanticweb.org/gianpietro/ontologies/2022/6/untitled-ontology-39"/>
    


    <!-- 
    ///////////////////////////////////////////////////////////////////////////////////////
    //
    // Object Properties
    //
    ///////////////////////////////////////////////////////////////////////////////////////
     -->

    


    <!-- http://www.semanticweb.org/gianpietro/ontologies/2022/6/untitled-ontology-39#adopt -->

    <owl:ObjectProperty rdf:about="http://www.semanticweb.org/gianpietro/ontologies/2022/6/untitled-ontology-39#adopt">
        <rdfs:subPropertyOf rdf:resource="http://www.semanticweb.org/gianpietro/ontologies/2022/6/untitled-ontology-39#article5Properties"/>
    </owl:ObjectProperty>
    


    <!-- http://www.semanticweb.org/gianpietro/ontologies/2022/6/untitled-ontology-39#adoptPolicies -->

    <owl:ObjectProperty rdf:about="http://www.semanticweb.org/gianpietro/ontologies/2022/6/untitled-ontology-39#adoptPolicies">
        <rdfs:subPropertyOf rdf:resource="http://www.semanticweb.org/gianpietro/ontologies/2022/6/untitled-ontology-39#article5Properties"/>
    </owl:ObjectProperty>
    


    <!-- http://www.semanticweb.org/gianpietro/ontologies/2022/6/untitled-ontology-39#article5Properties -->

    <owl:ObjectProperty rdf:about="http://www.semanticweb.org/gianpietro/ontologies/2022/6/untitled-ontology-39#article5Properties"/>
    


    <!-- http://www.semanticweb.org/gianpietro/ontologies/2022/6/untitled-ontology-39#assess -->

    <owl:ObjectProperty rdf:about="http://www.semanticweb.org/gianpietro/ontologies/2022/6/untitled-ontology-39#assess">
        <rdfs:subPropertyOf rdf:resource="http://www.semanticweb.org/gianpietro/ontologies/2022/6/untitled-ontology-39#article5Properties"/>
    </owl:ObjectProperty>
    


    <!-- http://www.semanticweb.org/gianpietro/ontologies/2022/6/untitled-ontology-39#assessPeriodically -->

    <owl:ObjectProperty rdf:about="http://www.semanticweb.org/gianpietro/ontologies/2022/6/untitled-ontology-39#assessPeriodically">
        <rdfs:subPropertyOf rdf:resource="http://www.semanticweb.org/gianpietro/ontologies/2022/6/untitled-ontology-39#article5Properties"/>
    </owl:ObjectProperty>
    


    <!-- http://www.semanticweb.org/gianpietro/ontologies/2022/6/untitled-ontology-39#hasSecurityProperty -->

    <owl:ObjectProperty rdf:about="http://www.semanticweb.org/gianpietro/ontologies/2022/6/untitled-ontology-39#hasSecurityProperty"/>
    


    <!-- http://www.semanticweb.org/gianpietro/ontologies/2022/6/untitled-ontology-39#include -->

    <owl:ObjectProperty rdf:about="http://www.semanticweb.org/gianpietro/ontologies/2022/6/untitled-ontology-39#include">
        <rdfs:subPropertyOf rdf:resource="http://www.semanticweb.org/gianpietro/ontologies/2022/6/untitled-ontology-39#article5Properties"/>
    </owl:ObjectProperty>
    


    <!-- http://www.semanticweb.org/gianpietro/ontologies/2022/6/untitled-ontology-39#isAnEntity -->

    <owl:ObjectProperty rdf:about="http://www.semanticweb.org/gianpietro/ontologies/2022/6/untitled-ontology-39#isAnEntity"/>
    


    <!-- http://www.semanticweb.org/gianpietro/ontologies/2022/6/untitled-ontology-39#isEssentialEntity -->

    <owl:ObjectProperty rdf:about="http://www.semanticweb.org/gianpietro/ontologies/2022/6/untitled-ontology-39#isEssentialEntity">
        <rdfs:subPropertyOf rdf:resource="http://www.semanticweb.org/gianpietro/ontologies/2022/6/untitled-ontology-39#isAnEntity"/>
        <rdfs:domain rdf:resource="http://www.dmi.unict.it/oasis.owl#Agent"/>
        <rdfs:domain rdf:resource="http://www.semanticweb.org/gianpietro/ontologies/2022/6/untitled-ontology-39#Entity"/>
    </owl:ObjectProperty>
    


    <!-- http://www.semanticweb.org/gianpietro/ontologies/2022/6/untitled-ontology-39#isImportanEntity -->

    <owl:ObjectProperty rdf:about="http://www.semanticweb.org/gianpietro/ontologies/2022/6/untitled-ontology-39#isImportanEntity">
        <rdfs:subPropertyOf rdf:resource="http://www.semanticweb.org/gianpietro/ontologies/2022/6/untitled-ontology-39#isAnEntity"/>
    </owl:ObjectProperty>
    


    <!-- http://www.semanticweb.org/gianpietro/ontologies/2022/6/untitled-ontology-39#notify -->

    <owl:ObjectProperty rdf:about="http://www.semanticweb.org/gianpietro/ontologies/2022/6/untitled-ontology-39#notify">
        <rdfs:subPropertyOf rdf:resource="http://www.semanticweb.org/gianpietro/ontologies/2022/6/untitled-ontology-39#article5Properties"/>
    </owl:ObjectProperty>
    


    <!-- 
    ///////////////////////////////////////////////////////////////////////////////////////
    //
    // Classes
    //
    ///////////////////////////////////////////////////////////////////////////////////////
     -->

    


    <!-- http://www.dmi.unict.it/oasis.owl#Agent -->

    <owl:Class rdf:about="http://www.dmi.unict.it/oasis.owl#Agent">
        <rdfs:subClassOf rdf:resource="http://www.semanticweb.org/gianpietro/ontologies/2022/6/untitled-ontology-39#Actor"/>
    </owl:Class>
    


    <!-- http://www.dmi.unict.it/oasis.owl#Human -->

    <owl:Class rdf:about="http://www.dmi.unict.it/oasis.owl#Human">
        <rdfs:subClassOf rdf:resource="http://www.dmi.unict.it/oasis.owl#Agent"/>
    </owl:Class>
    


    <!-- http://www.dmi.unict.it/oasis.owl#MultiAgentSystem -->

    <owl:Class rdf:about="http://www.dmi.unict.it/oasis.owl#MultiAgentSystem">
        <rdfs:subClassOf rdf:resource="http://www.dmi.unict.it/oasis.owl#System"/>
    </owl:Class>
    


    <!-- http://www.dmi.unict.it/oasis.owl#Process -->

    <owl:Class rdf:about="http://www.dmi.unict.it/oasis.owl#Process"/>
    


    <!-- http://www.dmi.unict.it/oasis.owl#Service -->

    <owl:Class rdf:about="http://www.dmi.unict.it/oasis.owl#Service">
        <rdfs:subClassOf rdf:resource="http://www.semanticweb.org/gianpietro/ontologies/2022/6/untitled-ontology-39#Actor"/>
    </owl:Class>
    


    <!-- http://www.dmi.unict.it/oasis.owl#System -->

    <owl:Class rdf:about="http://www.dmi.unict.it/oasis.owl#System">
        <rdfs:subClassOf rdf:resource="http://www.semanticweb.org/gianpietro/ontologies/2022/6/untitled-ontology-39#Actor"/>
    </owl:Class>
    


    <!-- http://www.semanticweb.org/gianpietro/ontologies/2022/6/untitled-ontology-39#AcademicResearchSupportingPolicy -->

    <owl:Class rdf:about="http://www.semanticweb.org/gianpietro/ontologies/2022/6/untitled-ontology-39#AcademicResearchSupportingPolicy">
        <rdfs:subClassOf rdf:resource="http://www.semanticweb.org/gianpietro/ontologies/2022/6/untitled-ontology-39#Article5Policies"/>
        <rdfs:comment>A policy on supporting academic and research institutions to develop
cybersecurity tools and secure network infrastructure.</rdfs:comment>
    </owl:Class>
    


    <!-- http://www.semanticweb.org/gianpietro/ontologies/2022/6/untitled-ontology-39#Actor -->

    <owl:Class rdf:about="http://www.semanticweb.org/gianpietro/ontologies/2022/6/untitled-ontology-39#Actor"/>
    


    <!-- http://www.semanticweb.org/gianpietro/ontologies/2022/6/untitled-ontology-39#Article-5-Compliant -->

    <owl:Class rdf:about="http://www.semanticweb.org/gianpietro/ontologies/2022/6/untitled-ontology-39#Article-5-Compliant">
        <owl:equivalentClass rdf:resource="http://www.semanticweb.org/gianpietro/ontologies/2022/6/untitled-ontology-39#MemberState"/>
        <owl:equivalentClass rdf:resource="http://www.semanticweb.org/gianpietro/ontologies/2022/6/untitled-ontology-39#NationalCyberSecurityStrategy"/>
        <owl:equivalentClass>
            <owl:Class>
                <owl:intersectionOf rdf:parseType="Collection">
                    <owl:Restriction>
                        <owl:onProperty rdf:resource="http://www.semanticweb.org/gianpietro/ontologies/2022/6/untitled-ontology-39#adoptPolicies"/>
                        <owl:someValuesFrom rdf:resource="http://www.semanticweb.org/gianpietro/ontologies/2022/6/untitled-ontology-39#Article5Policies"/>
                    </owl:Restriction>
                    <owl:Restriction>
                        <owl:onProperty rdf:resource="http://www.semanticweb.org/gianpietro/ontologies/2022/6/untitled-ontology-39#include"/>
                        <owl:someValuesFrom rdf:resource="http://www.semanticweb.org/gianpietro/ontologies/2022/6/untitled-ontology-39#CybersecurityAuthoritiesActorsList"/>
                    </owl:Restriction>
                    <owl:Restriction>
                        <owl:onProperty rdf:resource="http://www.semanticweb.org/gianpietro/ontologies/2022/6/untitled-ontology-39#include"/>
                        <owl:someValuesFrom rdf:resource="http://www.semanticweb.org/gianpietro/ontologies/2022/6/untitled-ontology-39#CybersecurityStrategyObjectivesPriorities"/>
                    </owl:Restriction>
                    <owl:Restriction>
                        <owl:onProperty rdf:resource="http://www.semanticweb.org/gianpietro/ontologies/2022/6/untitled-ontology-39#include"/>
                        <owl:someValuesFrom rdf:resource="http://www.semanticweb.org/gianpietro/ontologies/2022/6/untitled-ontology-39#EnhancedCoordinationPolicyFramework"/>
                    </owl:Restriction>
                    <owl:Restriction>
                        <owl:onProperty rdf:resource="http://www.semanticweb.org/gianpietro/ontologies/2022/6/untitled-ontology-39#include"/>
                        <owl:someValuesFrom rdf:resource="http://www.semanticweb.org/gianpietro/ontologies/2022/6/untitled-ontology-39#GovernanceFramework"/>
                    </owl:Restriction>
                    <owl:Restriction>
                        <owl:onProperty rdf:resource="http://www.semanticweb.org/gianpietro/ontologies/2022/6/untitled-ontology-39#include"/>
                        <owl:someValuesFrom rdf:resource="http://www.semanticweb.org/gianpietro/ontologies/2022/6/untitled-ontology-39#MeasuresIdentification"/>
                    </owl:Restriction>
                    <owl:Restriction>
                        <owl:onProperty rdf:resource="http://www.semanticweb.org/gianpietro/ontologies/2022/6/untitled-ontology-39#include"/>
                        <owl:someValuesFrom rdf:resource="http://www.semanticweb.org/gianpietro/ontologies/2022/6/untitled-ontology-39#RiskAssessment"/>
                    </owl:Restriction>
                    <owl:Restriction>
                        <owl:onProperty rdf:resource="http://www.semanticweb.org/gianpietro/ontologies/2022/6/untitled-ontology-39#notify"/>
                        <owl:someValuesFrom rdf:resource="http://www.semanticweb.org/gianpietro/ontologies/2022/6/untitled-ontology-39#NationalCyberSecurityStrategy"/>
                    </owl:Restriction>
                </owl:intersectionOf>
            </owl:Class>
        </owl:equivalentClass>
        <rdfs:subClassOf rdf:resource="http://www.semanticweb.org/gianpietro/ontologies/2022/6/untitled-ontology-39#Articles"/>
    </owl:Class>
    


    <!-- http://www.semanticweb.org/gianpietro/ontologies/2022/6/untitled-ontology-39#Article5Policies -->

    <owl:Class rdf:about="http://www.semanticweb.org/gianpietro/ontologies/2022/6/untitled-ontology-39#Article5Policies"/>
    


    <!-- http://www.semanticweb.org/gianpietro/ontologies/2022/6/untitled-ontology-39#Articles -->

    <owl:Class rdf:about="http://www.semanticweb.org/gianpietro/ontologies/2022/6/untitled-ontology-39#Articles"/>
    


    <!-- http://www.semanticweb.org/gianpietro/ontologies/2022/6/untitled-ontology-39#CloudComputingService -->

    <owl:Class rdf:about="http://www.semanticweb.org/gianpietro/ontologies/2022/6/untitled-ontology-39#CloudComputingService">
        <rdfs:subClassOf rdf:resource="http://www.dmi.unict.it/oasis.owl#Service"/>
        <rdfs:comment>It means a digital service that enables on-demand
administration and broad remote access to a scalable and elastic pool of shareable
and distributed computing resources.</rdfs:comment>
    </owl:Class>
    


    <!-- http://www.semanticweb.org/gianpietro/ontologies/2022/6/untitled-ontology-39#ContentDeliveryNetwork -->

    <owl:Class rdf:about="http://www.semanticweb.org/gianpietro/ontologies/2022/6/untitled-ontology-39#ContentDeliveryNetwork">
        <rdfs:subClassOf rdf:resource="http://www.dmi.unict.it/oasis.owl#MultiAgentSystem"/>
        <rdfs:comment>It means a network of geographically distributed servers for
the purpose of ensuring high availability, accessibility or fast delivery of digital
content and services to internet users on behalf of content and service providers.</rdfs:comment>
    </owl:Class>
    


    <!-- http://www.semanticweb.org/gianpietro/ontologies/2022/6/untitled-ontology-39#CoordinatedVulnerabilityDisclosurePolicy -->

    <owl:Class rdf:about="http://www.semanticweb.org/gianpietro/ontologies/2022/6/untitled-ontology-39#CoordinatedVulnerabilityDisclosurePolicy">
        <rdfs:subClassOf rdf:resource="http://www.semanticweb.org/gianpietro/ontologies/2022/6/untitled-ontology-39#Article5Policies"/>
        <rdfs:comment>A policy to promote and facilitate coordinated vulnerability disclosure within
the meaning of Article 6 of NIS directive.</rdfs:comment>
    </owl:Class>
    


    <!-- http://www.semanticweb.org/gianpietro/ontologies/2022/6/untitled-ontology-39#CyberThreat -->

    <owl:Class rdf:about="http://www.semanticweb.org/gianpietro/ontologies/2022/6/untitled-ontology-39#CyberThreat">
        <rdfs:subClassOf rdf:resource="http://www.semanticweb.org/gianpietro/ontologies/2022/6/untitled-ontology-39#Threat"/>
        <rdfs:comment>It means a cyber threat within the meaning Article 2(8) of Regulation
(EU) 2019/881.</rdfs:comment>
    </owl:Class>
    


    <!-- http://www.semanticweb.org/gianpietro/ontologies/2022/6/untitled-ontology-39#Cybersecurity -->

    <owl:Class rdf:about="http://www.semanticweb.org/gianpietro/ontologies/2022/6/untitled-ontology-39#Cybersecurity">
        <rdfs:subClassOf rdf:resource="http://www.semanticweb.org/gianpietro/ontologies/2022/6/untitled-ontology-39#Property"/>
        <rdfs:comment>It means cybersecurity within the meaning of Article 2(1) of Regulation
(EU) 2019/881 of the European Parliament and of the Council.</rdfs:comment>
    </owl:Class>
    


    <!-- http://www.semanticweb.org/gianpietro/ontologies/2022/6/untitled-ontology-39#CybersecurityAuthoritiesActorsList -->

    <owl:Class rdf:about="http://www.semanticweb.org/gianpietro/ontologies/2022/6/untitled-ontology-39#CybersecurityAuthoritiesActorsList">
        <rdfs:subClassOf rdf:resource="http://www.semanticweb.org/gianpietro/ontologies/2022/6/untitled-ontology-39#Actor"/>
        <rdfs:comment>List of cybertsecurity authorities and actors.</rdfs:comment>
    </owl:Class>
    


    <!-- http://www.semanticweb.org/gianpietro/ontologies/2022/6/untitled-ontology-39#CybersecurityInformationSharingPolicy -->

    <owl:Class rdf:about="http://www.semanticweb.org/gianpietro/ontologies/2022/6/untitled-ontology-39#CybersecurityInformationSharingPolicy">
        <rdfs:subClassOf rdf:resource="http://www.semanticweb.org/gianpietro/ontologies/2022/6/untitled-ontology-39#Article5Policies"/>
        <rdfs:comment>A policy, relevant procedures and appropriate information-sharing tools to
support voluntary cybersecurity information sharing between companies in
compliance with Union law.</rdfs:comment>
    </owl:Class>
    


    <!-- http://www.semanticweb.org/gianpietro/ontologies/2022/6/untitled-ontology-39#CybersecuritySkillsPromotingPolicy -->

    <owl:Class rdf:about="http://www.semanticweb.org/gianpietro/ontologies/2022/6/untitled-ontology-39#CybersecuritySkillsPromotingPolicy">
        <rdfs:subClassOf rdf:resource="http://www.semanticweb.org/gianpietro/ontologies/2022/6/untitled-ontology-39#Article5Policies"/>
        <rdfs:comment>A policy on promoting and developing cybersecurity skills, awareness raising and research and development initiatives.</rdfs:comment>
    </owl:Class>
    


    <!-- http://www.semanticweb.org/gianpietro/ontologies/2022/6/untitled-ontology-39#CybersecurityStrategyObjectivesPriorities -->

    <owl:Class rdf:about="http://www.semanticweb.org/gianpietro/ontologies/2022/6/untitled-ontology-39#CybersecurityStrategyObjectivesPriorities">
        <rdfs:subClassOf rdf:resource="http://www.semanticweb.org/gianpietro/ontologies/2022/6/untitled-ontology-39#Procedure"/>
    </owl:Class>
    


    <!-- http://www.semanticweb.org/gianpietro/ontologies/2022/6/untitled-ontology-39#DNS -->

    <owl:Class rdf:about="http://www.semanticweb.org/gianpietro/ontologies/2022/6/untitled-ontology-39#DNS">
        <rdfs:subClassOf rdf:resource="http://www.dmi.unict.it/oasis.owl#MultiAgentSystem"/>
        <rdfs:comment>It means a hierarchical distributed naming system which
allows end-users to reach services and resources on the internet.</rdfs:comment>
    </owl:Class>
    


    <!-- http://www.semanticweb.org/gianpietro/ontologies/2022/6/untitled-ontology-39#DNSServiceProvider -->

    <owl:Class rdf:about="http://www.semanticweb.org/gianpietro/ontologies/2022/6/untitled-ontology-39#DNSServiceProvider">
        <rdfs:subClassOf rdf:resource="http://www.dmi.unict.it/oasis.owl#Service"/>
        <rdfs:comment>It means an entity that provides recursive or authoritative
domain name resolution services to internet end-users and other DNS service
providers.</rdfs:comment>
    </owl:Class>
    


    <!-- http://www.semanticweb.org/gianpietro/ontologies/2022/6/untitled-ontology-39#DataCentre -->

    <owl:Class rdf:about="http://www.semanticweb.org/gianpietro/ontologies/2022/6/untitled-ontology-39#DataCentre">
        <rdfs:subClassOf rdf:resource="http://www.dmi.unict.it/oasis.owl#Service"/>
        <rdfs:comment>It means a service that encompasses structures, or groups of
structures, dedicated to the centralised accommodation, interconnection and
operation of information technology and network equipment providing data storage,
processing and transport services together with all the facilities and infrastructures
for power distribution and environmental control</rdfs:comment>
    </owl:Class>
    


    <!-- http://www.semanticweb.org/gianpietro/ontologies/2022/6/untitled-ontology-39#DigitalService -->

    <owl:Class rdf:about="http://www.semanticweb.org/gianpietro/ontologies/2022/6/untitled-ontology-39#DigitalService">
        <rdfs:subClassOf rdf:resource="http://www.dmi.unict.it/oasis.owl#Service"/>
        <rdfs:comment>It means a service within the meaning of Article 1(1)(b) of Directive
(EU) 2015/1535 of the European Parliament and of the Council.</rdfs:comment>
    </owl:Class>
    


    <!-- http://www.semanticweb.org/gianpietro/ontologies/2022/6/untitled-ontology-39#EnhancedCoordinationPolicyFramework -->

    <owl:Class rdf:about="http://www.semanticweb.org/gianpietro/ontologies/2022/6/untitled-ontology-39#EnhancedCoordinationPolicyFramework">
        <rdfs:subClassOf rdf:resource="http://www.semanticweb.org/gianpietro/ontologies/2022/6/untitled-ontology-39#Frameworks"/>
        <rdfs:comment>A framework for enhanced coordination policy between member states.</rdfs:comment>
    </owl:Class>
    


    <!-- http://www.semanticweb.org/gianpietro/ontologies/2022/6/untitled-ontology-39#Entity -->

    <owl:Class rdf:about="http://www.semanticweb.org/gianpietro/ontologies/2022/6/untitled-ontology-39#Entity">
        <rdfs:comment>It means any natural or legal person created and recognised as such under the
national law of its place of establishment, which may, acting under its own name,
exercise rights and be subject to obligations.</rdfs:comment>
    </owl:Class>
    


    <!-- http://www.semanticweb.org/gianpietro/ontologies/2022/6/untitled-ontology-39#Event -->

    <owl:Class rdf:about="http://www.semanticweb.org/gianpietro/ontologies/2022/6/untitled-ontology-39#Event"/>
    


    <!-- http://www.semanticweb.org/gianpietro/ontologies/2022/6/untitled-ontology-39#Frameworks -->

    <owl:Class rdf:about="http://www.semanticweb.org/gianpietro/ontologies/2022/6/untitled-ontology-39#Frameworks"/>
    


    <!-- http://www.semanticweb.org/gianpietro/ontologies/2022/6/untitled-ontology-39#GovernanceFramework -->

    <owl:Class rdf:about="http://www.semanticweb.org/gianpietro/ontologies/2022/6/untitled-ontology-39#GovernanceFramework">
        <rdfs:subClassOf rdf:resource="http://www.semanticweb.org/gianpietro/ontologies/2022/6/untitled-ontology-39#Frameworks"/>
    </owl:Class>
    


    <!-- http://www.semanticweb.org/gianpietro/ontologies/2022/6/untitled-ontology-39#Incident -->

    <owl:Class rdf:about="http://www.semanticweb.org/gianpietro/ontologies/2022/6/untitled-ontology-39#Incident">
        <rdfs:subClassOf rdf:resource="http://www.semanticweb.org/gianpietro/ontologies/2022/6/untitled-ontology-39#Event"/>
        <rdfs:comment>It means any event compromising the availability, authenticity, integrity or
confidentiality of stored, transmitted or processed data or of the related services
offered by, or accessible via, network and information systems.</rdfs:comment>
    </owl:Class>
    


    <!-- http://www.semanticweb.org/gianpietro/ontologies/2022/6/untitled-ontology-39#IncidentHandling -->

    <owl:Class rdf:about="http://www.semanticweb.org/gianpietro/ontologies/2022/6/untitled-ontology-39#IncidentHandling">
        <rdfs:subClassOf rdf:resource="http://www.semanticweb.org/gianpietro/ontologies/2022/6/untitled-ontology-39#Procedure"/>
        <rdfs:comment>It means all actions and procedures aiming at detection, analysis
and containment of and a response to an incident.</rdfs:comment>
    </owl:Class>
    


    <!-- http://www.semanticweb.org/gianpietro/ontologies/2022/6/untitled-ontology-39#Institution -->

    <owl:Class rdf:about="http://www.semanticweb.org/gianpietro/ontologies/2022/6/untitled-ontology-39#Institution">
        <rdfs:subClassOf rdf:resource="http://www.semanticweb.org/gianpietro/ontologies/2022/6/untitled-ontology-39#Actor"/>
    </owl:Class>
    


    <!-- http://www.semanticweb.org/gianpietro/ontologies/2022/6/untitled-ontology-39#InternetExchangePoint -->

    <owl:Class rdf:about="http://www.semanticweb.org/gianpietro/ontologies/2022/6/untitled-ontology-39#InternetExchangePoint">
        <rdfs:subClassOf rdf:resource="http://www.dmi.unict.it/oasis.owl#MultiAgentSystem"/>
        <rdfs:comment>It means a network facility which enables the
interconnection of more than two independent networks (autonomous systems),
primarily for the purpose of facilitating the exchange of internet traffic.</rdfs:comment>
    </owl:Class>
    


    <!-- http://www.semanticweb.org/gianpietro/ontologies/2022/6/untitled-ontology-39#MeasuresIdentification -->

    <owl:Class rdf:about="http://www.semanticweb.org/gianpietro/ontologies/2022/6/untitled-ontology-39#MeasuresIdentification">
        <rdfs:subClassOf rdf:resource="http://www.semanticweb.org/gianpietro/ontologies/2022/6/untitled-ontology-39#RiskAssessment"/>
    </owl:Class>
    


    <!-- http://www.semanticweb.org/gianpietro/ontologies/2022/6/untitled-ontology-39#MemberState -->

    <owl:Class rdf:about="http://www.semanticweb.org/gianpietro/ontologies/2022/6/untitled-ontology-39#MemberState">
        <rdfs:subClassOf rdf:resource="http://www.semanticweb.org/gianpietro/ontologies/2022/6/untitled-ontology-39#Institution"/>
        <rdfs:comment>State member of european union.</rdfs:comment>
    </owl:Class>
    


    <!-- http://www.semanticweb.org/gianpietro/ontologies/2022/6/untitled-ontology-39#NationalCyberSecurityStrategy -->

    <owl:Class rdf:about="http://www.semanticweb.org/gianpietro/ontologies/2022/6/untitled-ontology-39#NationalCyberSecurityStrategy">
        <rdfs:subClassOf rdf:resource="http://www.semanticweb.org/gianpietro/ontologies/2022/6/untitled-ontology-39#Procedure"/>
    </owl:Class>
    


    <!-- http://www.semanticweb.org/gianpietro/ontologies/2022/6/untitled-ontology-39#NetworkInformationSystem -->

    <owl:Class rdf:about="http://www.semanticweb.org/gianpietro/ontologies/2022/6/untitled-ontology-39#NetworkInformationSystem">
        <rdfs:subClassOf rdf:resource="http://www.dmi.unict.it/oasis.owl#System"/>
    </owl:Class>
    


    <!-- http://www.semanticweb.org/gianpietro/ontologies/2022/6/untitled-ontology-39#NetworkInformationSystemSecurity -->

    <owl:Class rdf:about="http://www.semanticweb.org/gianpietro/ontologies/2022/6/untitled-ontology-39#NetworkInformationSystemSecurity">
        <rdfs:subClassOf rdf:resource="http://www.semanticweb.org/gianpietro/ontologies/2022/6/untitled-ontology-39#Property"/>
        <rdfs:comment>It means the ability of network and information systems to resist, at a given level of confidence, any action that compromises the availability, authenticity, integrity or confidentiality of stored or transmitted or processed data or the related services offered by, or accessible via, those network and information systems.</rdfs:comment>
        <rdfs:comment>Security of information and network systems</rdfs:comment>
    </owl:Class>
    


    <!-- http://www.semanticweb.org/gianpietro/ontologies/2022/6/untitled-ontology-39#OnlineMarketplace -->

    <owl:Class rdf:about="http://www.semanticweb.org/gianpietro/ontologies/2022/6/untitled-ontology-39#OnlineMarketplace">
        <rdfs:subClassOf rdf:resource="http://www.dmi.unict.it/oasis.owl#Service"/>
        <rdfs:comment>It means a digital service within the meaning of Article 2 point
(n) of Directive 2005/29/EC of the European Parliament and of the Council.</rdfs:comment>
    </owl:Class>
    


    <!-- http://www.semanticweb.org/gianpietro/ontologies/2022/6/untitled-ontology-39#OnlineSearchEngine -->

    <owl:Class rdf:about="http://www.semanticweb.org/gianpietro/ontologies/2022/6/untitled-ontology-39#OnlineSearchEngine">
        <rdfs:subClassOf rdf:resource="http://www.dmi.unict.it/oasis.owl#Service"/>
        <rdfs:comment>It means a digital service within the meaning of Article 2(5) of
Regulation (EU) 2019/1150 of the European Parliament and of the Council.</rdfs:comment>
    </owl:Class>
    


    <!-- http://www.semanticweb.org/gianpietro/ontologies/2022/6/untitled-ontology-39#OpenInternetIntegrityAvailabilityPolicy -->

    <owl:Class rdf:about="http://www.semanticweb.org/gianpietro/ontologies/2022/6/untitled-ontology-39#OpenInternetIntegrityAvailabilityPolicy">
        <rdfs:subClassOf rdf:resource="http://www.semanticweb.org/gianpietro/ontologies/2022/6/untitled-ontology-39#Article5Policies"/>
        <rdfs:comment>A policy related to sustaining the general availability and integrity of the public
core of the open internet.</rdfs:comment>
    </owl:Class>
    


    <!-- http://www.semanticweb.org/gianpietro/ontologies/2022/6/untitled-ontology-39#Procedure -->

    <owl:Class rdf:about="http://www.semanticweb.org/gianpietro/ontologies/2022/6/untitled-ontology-39#Procedure"/>
    


    <!-- http://www.semanticweb.org/gianpietro/ontologies/2022/6/untitled-ontology-39#Property -->

    <owl:Class rdf:about="http://www.semanticweb.org/gianpietro/ontologies/2022/6/untitled-ontology-39#Property"/>
    


    <!-- http://www.semanticweb.org/gianpietro/ontologies/2022/6/untitled-ontology-39#PublicAdministration -->

    <owl:Class rdf:about="http://www.semanticweb.org/gianpietro/ontologies/2022/6/untitled-ontology-39#PublicAdministration">
        <rdfs:subClassOf rdf:resource="http://www.semanticweb.org/gianpietro/ontologies/2022/6/untitled-ontology-39#Entity"/>
        <rdfs:comment>It means an entity in a Member State that complies with
the following criteria:
(a)it is established for the purpose of meeting needs in the general interest and
does not have an industrial or commercial character;
(b)it has legal personality;
(c)it is financed, for the most part, by the State, regional authority, or by other
bodies governed by public law; or it is subject to management supervision by
those authorities or bodies; or it has an administrative, managerial or
supervisory board, more than half of whose members are appointed by the
State, regional authorities, or by other bodies governed by public law;
(d)it has the power to address to natural or legal persons administrative or
regulatory decisions affecting their rights in the cross-border movement of
persons, goods, services or capital.</rdfs:comment>
    </owl:Class>
    


    <!-- http://www.semanticweb.org/gianpietro/ontologies/2022/6/untitled-ontology-39#Representative -->

    <owl:Class rdf:about="http://www.semanticweb.org/gianpietro/ontologies/2022/6/untitled-ontology-39#Representative">
        <rdfs:subClassOf rdf:resource="http://www.dmi.unict.it/oasis.owl#Human"/>
        <rdfs:comment>It means any natural or legal person established in the Union explicitly
designated to act on behalf of i) a DNS service provider, a top-level domain (TLD)
name registry, a cloud computing service provider, a data centre service provider, a
content delivery network provider.</rdfs:comment>
    </owl:Class>
    


    <!-- http://www.semanticweb.org/gianpietro/ontologies/2022/6/untitled-ontology-39#RiskAssessment -->

    <owl:Class rdf:about="http://www.semanticweb.org/gianpietro/ontologies/2022/6/untitled-ontology-39#RiskAssessment"/>
    


    <!-- http://www.semanticweb.org/gianpietro/ontologies/2022/6/untitled-ontology-39#SMEThreatResiliencePolicy -->

    <owl:Class rdf:about="http://www.semanticweb.org/gianpietro/ontologies/2022/6/untitled-ontology-39#SMEThreatResiliencePolicy">
        <rdfs:subClassOf rdf:resource="http://www.semanticweb.org/gianpietro/ontologies/2022/6/untitled-ontology-39#Article5Policies"/>
        <rdfs:comment>A policy addressing specific needs of SMEs, in particular those excluded from
the scope of this Directive, in relation to guidance and support in improving
their resilience to cybersecurity threats.</rdfs:comment>
    </owl:Class>
    


    <!-- http://www.semanticweb.org/gianpietro/ontologies/2022/6/untitled-ontology-39#SocialNetworkPlatform -->

    <owl:Class rdf:about="http://www.semanticweb.org/gianpietro/ontologies/2022/6/untitled-ontology-39#SocialNetworkPlatform">
        <rdfs:subClassOf rdf:resource="http://www.semanticweb.org/gianpietro/ontologies/2022/6/untitled-ontology-39#NetworkInformationSystem"/>
        <rdfs:comment>It means a platform that enables end-users to
connect, share, discover and communicate with each other across multiple devices.</rdfs:comment>
    </owl:Class>
    


    <!-- http://www.semanticweb.org/gianpietro/ontologies/2022/6/untitled-ontology-39#Standard -->

    <owl:Class rdf:about="http://www.semanticweb.org/gianpietro/ontologies/2022/6/untitled-ontology-39#Standard">
        <rdfs:subClassOf rdf:resource="http://www.semanticweb.org/gianpietro/ontologies/2022/6/untitled-ontology-39#Procedure"/>
        <rdfs:comment>It means a standard within the meaning of Article 2(1) of Regulation (EU)
No 1025/2012 of the European Parliament and of the Council.</rdfs:comment>
    </owl:Class>
    


    <!-- http://www.semanticweb.org/gianpietro/ontologies/2022/6/untitled-ontology-39#SupplychainPolicy -->

    <owl:Class rdf:about="http://www.semanticweb.org/gianpietro/ontologies/2022/6/untitled-ontology-39#SupplychainPolicy">
        <rdfs:subClassOf rdf:resource="http://www.semanticweb.org/gianpietro/ontologies/2022/6/untitled-ontology-39#Article5Policies"/>
        <rdfs:comment>A policy addressing cybersecurity in the supply chain for ICT products and
services used by essential and important entities for the provision of their
services.</rdfs:comment>
    </owl:Class>
    


    <!-- http://www.semanticweb.org/gianpietro/ontologies/2022/6/untitled-ontology-39#TechnicalSpecification -->

    <owl:Class rdf:about="http://www.semanticweb.org/gianpietro/ontologies/2022/6/untitled-ontology-39#TechnicalSpecification">
        <rdfs:subClassOf rdf:resource="http://www.semanticweb.org/gianpietro/ontologies/2022/6/untitled-ontology-39#Procedure"/>
        <rdfs:comment>It means a technical specification within the meaning of Article 2(4) of Regulation (EU) No 1025/2012.</rdfs:comment>
    </owl:Class>
    


    <!-- http://www.semanticweb.org/gianpietro/ontologies/2022/6/untitled-ontology-39#Threat -->

    <owl:Class rdf:about="http://www.semanticweb.org/gianpietro/ontologies/2022/6/untitled-ontology-39#Threat"/>
    


    <!-- http://www.semanticweb.org/gianpietro/ontologies/2022/6/untitled-ontology-39#TopLevelDomainNameRegistry -->

    <owl:Class rdf:about="http://www.semanticweb.org/gianpietro/ontologies/2022/6/untitled-ontology-39#TopLevelDomainNameRegistry">
        <rdfs:subClassOf rdf:resource="http://www.semanticweb.org/gianpietro/ontologies/2022/6/untitled-ontology-39#Entity"/>
        <rdfs:comment>It means an entity which has been delegated a specific TLD and is responsible for administering the TLD including the registration of domain names under the TLD and the technical operation of the TLD, including the operation of its name servers, the maintenance of its databases and the distribution of TLD zone files across name servers.</rdfs:comment>
    </owl:Class>
    


    <!-- http://www.semanticweb.org/gianpietro/ontologies/2022/6/untitled-ontology-39#Vulnerability -->

    <owl:Class rdf:about="http://www.semanticweb.org/gianpietro/ontologies/2022/6/untitled-ontology-39#Vulnerability">
        <rdfs:subClassOf rdf:resource="http://www.semanticweb.org/gianpietro/ontologies/2022/6/untitled-ontology-39#Weakness"/>
        <rdfs:comment>It means a weakness, susceptibility or flaw of an asset, system, process
or control that can be exploited by a cyber threat.</rdfs:comment>
    </owl:Class>
    


    <!-- http://www.semanticweb.org/gianpietro/ontologies/2022/6/untitled-ontology-39#Weakness -->

    <owl:Class rdf:about="http://www.semanticweb.org/gianpietro/ontologies/2022/6/untitled-ontology-39#Weakness"/>
    


    <!-- 
    ///////////////////////////////////////////////////////////////////////////////////////
    //
    // Individuals
    //
    ///////////////////////////////////////////////////////////////////////////////////////
     -->

    


    <!-- http://www.semanticweb.org/gianpietro/ontologies/2022/6/untitled-ontology-39#Article-5-Compliant -->

    <owl:NamedIndividual rdf:about="http://www.semanticweb.org/gianpietro/ontologies/2022/6/untitled-ontology-39#Article-5-Compliant">
        <adopt rdf:resource="http://www.semanticweb.org/gianpietro/ontologies/2022/6/untitled-ontology-39#NationalCyberSecurityStrategy"/>
        <adoptPolicies rdf:resource="http://www.semanticweb.org/gianpietro/ontologies/2022/6/untitled-ontology-39#Article5Policies"/>
        <assessPeriodically rdf:resource="http://www.semanticweb.org/gianpietro/ontologies/2022/6/untitled-ontology-39#NationalCyberSecurityStrategy"/>
        <include rdf:resource="http://www.semanticweb.org/gianpietro/ontologies/2022/6/untitled-ontology-39#CoordinationPolicyFramework"/>
        <include rdf:resource="http://www.semanticweb.org/gianpietro/ontologies/2022/6/untitled-ontology-39#CybersecurityActorsAndAuthorities"/>
        <include rdf:resource="http://www.semanticweb.org/gianpietro/ontologies/2022/6/untitled-ontology-39#GovernanceFramework"/>
        <include rdf:resource="http://www.semanticweb.org/gianpietro/ontologies/2022/6/untitled-ontology-39#IncidentsMeasuresIdentification"/>
        <include rdf:resource="http://www.semanticweb.org/gianpietro/ontologies/2022/6/untitled-ontology-39#ObjectivesPrioritiesDefinition"/>
        <include rdf:resource="http://www.semanticweb.org/gianpietro/ontologies/2022/6/untitled-ontology-39#RiskAssessment"/>
        <notify rdf:resource="http://www.semanticweb.org/gianpietro/ontologies/2022/6/untitled-ontology-39#NationalCyberSecurityStrategy"/>
    </owl:NamedIndividual>
    


    <!-- http://www.semanticweb.org/gianpietro/ontologies/2022/6/untitled-ontology-39#Article-5-Not-Compliant -->

    <owl:NamedIndividual rdf:about="http://www.semanticweb.org/gianpietro/ontologies/2022/6/untitled-ontology-39#Article-5-Not-Compliant">
        <adoptPolicies rdf:resource="http://www.semanticweb.org/gianpietro/ontologies/2022/6/untitled-ontology-39#CybersecuritySkillsPromoting"/>
    </owl:NamedIndividual>
    


    <!-- http://www.semanticweb.org/gianpietro/ontologies/2022/6/untitled-ontology-39#Article5Policies -->

    <owl:NamedIndividual rdf:about="http://www.semanticweb.org/gianpietro/ontologies/2022/6/untitled-ontology-39#Article5Policies">
        <rdf:type rdf:resource="http://www.semanticweb.org/gianpietro/ontologies/2022/6/untitled-ontology-39#Article5Policies"/>
    </owl:NamedIndividual>
    


    <!-- http://www.semanticweb.org/gianpietro/ontologies/2022/6/untitled-ontology-39#CoordinatedVulnerabilityDisclosure -->

    <owl:NamedIndividual rdf:about="http://www.semanticweb.org/gianpietro/ontologies/2022/6/untitled-ontology-39#CoordinatedVulnerabilityDisclosure">
        <rdf:type rdf:resource="http://www.semanticweb.org/gianpietro/ontologies/2022/6/untitled-ontology-39#CoordinatedVulnerabilityDisclosurePolicy"/>
    </owl:NamedIndividual>
    


    <!-- http://www.semanticweb.org/gianpietro/ontologies/2022/6/untitled-ontology-39#CoordinationPolicyFramework -->

    <owl:NamedIndividual rdf:about="http://www.semanticweb.org/gianpietro/ontologies/2022/6/untitled-ontology-39#CoordinationPolicyFramework">
        <rdf:type rdf:resource="http://www.semanticweb.org/gianpietro/ontologies/2022/6/untitled-ontology-39#EnhancedCoordinationPolicyFramework"/>
    </owl:NamedIndividual>
    


    <!-- http://www.semanticweb.org/gianpietro/ontologies/2022/6/untitled-ontology-39#CybersecurityActorsAndAuthorities -->

    <owl:NamedIndividual rdf:about="http://www.semanticweb.org/gianpietro/ontologies/2022/6/untitled-ontology-39#CybersecurityActorsAndAuthorities">
        <rdf:type rdf:resource="http://www.semanticweb.org/gianpietro/ontologies/2022/6/untitled-ontology-39#CybersecurityAuthoritiesActorsList"/>
    </owl:NamedIndividual>
    


    <!-- http://www.semanticweb.org/gianpietro/ontologies/2022/6/untitled-ontology-39#CybersecurityResearchSupporting -->

    <owl:NamedIndividual rdf:about="http://www.semanticweb.org/gianpietro/ontologies/2022/6/untitled-ontology-39#CybersecurityResearchSupporting">
        <rdf:type rdf:resource="http://www.semanticweb.org/gianpietro/ontologies/2022/6/untitled-ontology-39#AcademicResearchSupportingPolicy"/>
    </owl:NamedIndividual>
    


    <!-- http://www.semanticweb.org/gianpietro/ontologies/2022/6/untitled-ontology-39#CybersecuritySkillsPromoting -->

    <owl:NamedIndividual rdf:about="http://www.semanticweb.org/gianpietro/ontologies/2022/6/untitled-ontology-39#CybersecuritySkillsPromoting">
        <rdf:type rdf:resource="http://www.semanticweb.org/gianpietro/ontologies/2022/6/untitled-ontology-39#CybersecuritySkillsPromotingPolicy"/>
    </owl:NamedIndividual>
    


    <!-- http://www.semanticweb.org/gianpietro/ontologies/2022/6/untitled-ontology-39#CybersecuritySupplyChainAddressing -->

    <owl:NamedIndividual rdf:about="http://www.semanticweb.org/gianpietro/ontologies/2022/6/untitled-ontology-39#CybersecuritySupplyChainAddressing">
        <rdf:type rdf:resource="http://www.semanticweb.org/gianpietro/ontologies/2022/6/untitled-ontology-39#SupplychainPolicy"/>
    </owl:NamedIndividual>
    


    <!-- http://www.semanticweb.org/gianpietro/ontologies/2022/6/untitled-ontology-39#GovernanceFramework -->

    <owl:NamedIndividual rdf:about="http://www.semanticweb.org/gianpietro/ontologies/2022/6/untitled-ontology-39#GovernanceFramework">
        <rdf:type rdf:resource="http://www.semanticweb.org/gianpietro/ontologies/2022/6/untitled-ontology-39#GovernanceFramework"/>
    </owl:NamedIndividual>
    


    <!-- http://www.semanticweb.org/gianpietro/ontologies/2022/6/untitled-ontology-39#IncidentsMeasuresIdentification -->

    <owl:NamedIndividual rdf:about="http://www.semanticweb.org/gianpietro/ontologies/2022/6/untitled-ontology-39#IncidentsMeasuresIdentification">
        <rdf:type rdf:resource="http://www.semanticweb.org/gianpietro/ontologies/2022/6/untitled-ontology-39#MeasuresIdentification"/>
    </owl:NamedIndividual>
    


    <!-- http://www.semanticweb.org/gianpietro/ontologies/2022/6/untitled-ontology-39#InformationSharing -->

    <owl:NamedIndividual rdf:about="http://www.semanticweb.org/gianpietro/ontologies/2022/6/untitled-ontology-39#InformationSharing">
        <rdf:type rdf:resource="http://www.semanticweb.org/gianpietro/ontologies/2022/6/untitled-ontology-39#CybersecurityInformationSharingPolicy"/>
    </owl:NamedIndividual>
    


    <!-- http://www.semanticweb.org/gianpietro/ontologies/2022/6/untitled-ontology-39#NationalCyberSecurityStrategy -->

    <owl:NamedIndividual rdf:about="http://www.semanticweb.org/gianpietro/ontologies/2022/6/untitled-ontology-39#NationalCyberSecurityStrategy">
        <rdf:type rdf:resource="http://www.semanticweb.org/gianpietro/ontologies/2022/6/untitled-ontology-39#NationalCyberSecurityStrategy"/>
        <include rdf:resource="http://www.semanticweb.org/gianpietro/ontologies/2022/6/untitled-ontology-39#CoordinationPolicyFramework"/>
        <include rdf:resource="http://www.semanticweb.org/gianpietro/ontologies/2022/6/untitled-ontology-39#CybersecurityActorsAndAuthorities"/>
        <include rdf:resource="http://www.semanticweb.org/gianpietro/ontologies/2022/6/untitled-ontology-39#GovernanceFramework"/>
        <include rdf:resource="http://www.semanticweb.org/gianpietro/ontologies/2022/6/untitled-ontology-39#IncidentsMeasuresIdentification"/>
        <include rdf:resource="http://www.semanticweb.org/gianpietro/ontologies/2022/6/untitled-ontology-39#ObjectivesPrioritiesDefinition"/>
    </owl:NamedIndividual>
    


    <!-- http://www.semanticweb.org/gianpietro/ontologies/2022/6/untitled-ontology-39#ObjectivesPrioritiesDefinition -->

    <owl:NamedIndividual rdf:about="http://www.semanticweb.org/gianpietro/ontologies/2022/6/untitled-ontology-39#ObjectivesPrioritiesDefinition">
        <rdf:type rdf:resource="http://www.semanticweb.org/gianpietro/ontologies/2022/6/untitled-ontology-39#CybersecurityStrategyObjectivesPriorities"/>
    </owl:NamedIndividual>
    


    <!-- http://www.semanticweb.org/gianpietro/ontologies/2022/6/untitled-ontology-39#OpenInternetIntegrityAvailabilitySustanance -->

    <owl:NamedIndividual rdf:about="http://www.semanticweb.org/gianpietro/ontologies/2022/6/untitled-ontology-39#OpenInternetIntegrityAvailabilitySustanance">
        <rdf:type rdf:resource="http://www.semanticweb.org/gianpietro/ontologies/2022/6/untitled-ontology-39#OpenInternetIntegrityAvailabilityPolicy"/>
    </owl:NamedIndividual>
    


    <!-- http://www.semanticweb.org/gianpietro/ontologies/2022/6/untitled-ontology-39#PublicProcurementCybersecurityRequirements -->

    <owl:NamedIndividual rdf:about="http://www.semanticweb.org/gianpietro/ontologies/2022/6/untitled-ontology-39#PublicProcurementCybersecurityRequirements"/>
    


    <!-- http://www.semanticweb.org/gianpietro/ontologies/2022/6/untitled-ontology-39#RelevantAssetsCybersecurityRisks -->

    <owl:NamedIndividual rdf:about="http://www.semanticweb.org/gianpietro/ontologies/2022/6/untitled-ontology-39#RelevantAssetsCybersecurityRisks"/>
    


    <!-- http://www.semanticweb.org/gianpietro/ontologies/2022/6/untitled-ontology-39#RiskAssessment -->

    <owl:NamedIndividual rdf:about="http://www.semanticweb.org/gianpietro/ontologies/2022/6/untitled-ontology-39#RiskAssessment">
        <rdf:type rdf:resource="http://www.semanticweb.org/gianpietro/ontologies/2022/6/untitled-ontology-39#RiskAssessment"/>
    </owl:NamedIndividual>
    


    <!-- http://www.semanticweb.org/gianpietro/ontologies/2022/6/untitled-ontology-39#SMEpolicy -->

    <owl:NamedIndividual rdf:about="http://www.semanticweb.org/gianpietro/ontologies/2022/6/untitled-ontology-39#SMEpolicy">
        <rdf:type rdf:resource="http://www.semanticweb.org/gianpietro/ontologies/2022/6/untitled-ontology-39#SMEThreatResiliencePolicy"/>
    </owl:NamedIndividual>
    


    <!-- 
    ///////////////////////////////////////////////////////////////////////////////////////
    //
    // Annotations
    //
    ///////////////////////////////////////////////////////////////////////////////////////
     -->

    <rdf:Description rdf:about="http://www.semanticweb.org/gianpietro/ontologies/2022/6/untitled-ontology-39#GovernanceFramework">
        <rdfs:comment>Provides a mechanism for senior management, as well as those at the operational level, to have a clear understanding and oversight of each other&apos;s expectations, objectives, performance, risk appetite, and reporting requirements.</rdfs:comment>
    </rdf:Description>
    <rdf:Description rdf:about="http://www.semanticweb.org/gianpietro/ontologies/2022/6/untitled-ontology-39#NationalCyberSecurityStrategy">
        <rdfs:comment>It means a coherent framework of a Member State providing strategic objectives and priorities on the security of network and information systems in that Member State.</rdfs:comment>
    </rdf:Description>
    <rdf:Description rdf:about="http://www.semanticweb.org/gianpietro/ontologies/2022/6/untitled-ontology-39#RiskAssessment">
        <rdfs:comment>It means the activity of evaluate assets and their weakness.</rdfs:comment>
    </rdf:Description>
</rdf:RDF>



<!-- Generated by the OWL API (version 4.5.9.2019-02-01T07:24:44Z) https://github.com/owlcs/owlapi -->

